nits

lib/prims.fst
@@ -497,7 +497,7 @@ logic type InductionHyp : Type -> Type
 assume val using_induction_hyp: 'a -> Lemma (ensures (InductionHyp 'a))
 assume val Assume: 'P:Type -> unit -> (y:unit{'P})
 assume val admit: unit -> Admit unit
-assume val admitP: 'P:Type -> unit -> Pure unit True (fun x -> 'P)
+assume val admitP: 'P:Type -> Pure unit True (fun x -> 'P)
 assume val Assert : 'P:Type -> unit -> Pure unit (requires $"assertion failed" 'P) (ensures \x -> True)
 assume val cut : 'P:Type -> Pure unit (requires $"assertion failed" 'P) (fun x -> 'P)
 assume val qintro: a:Type -> p:(a -> Type) -> (x:a -> Lemma (p x)) -> Lemma (forall (x:a). p x)
@@ -505,7 +505,8 @@ assume val failwith: string -> ALL.All 'a (fun h -> True) (fun h a h' -> h==h')
 assume val raise: exn -> 'a       (* TODO: refine with the Exn monad *)
 assume val pipe_right: 'a -> ('a -> 'b) -> 'b
 assume val pipe_left: ('a -> 'b) -> 'a -> 'b
-assume val ignore: 'a -> unit
+val ignore: 'a -> Tot unit
+let ignore x = ()
 assume val exit: int -> 'a
 assume val try_with: (unit -> 'a) -> (exn -> 'a) -> 'a
 assume logic val op_AmpAmp             : bool -> bool -> Tot bool
