examples/unit-tests/negative-tests.fst
@@ -57,9 +57,9 @@ assume DistinctXY: x <> y
 
 let test2 _ = assert (sel (upd (upd h x 0) y 1) y = 0) //should fail
 let test10 (x:ref int) (y:ref int) (h0:heap) (h1:heap) (h2:heap) =
-  admitP (h1 == concat h1 (restrict h0 (complement empty))) ();
-  admitP (h1 == upd h0 x 0) ();
-  admitP (~ (contains h1 y)) ();
+  admitP (h1 == concat h1 (restrict h0 (complement empty)));
+  admitP (h1 == upd h0 x 0);
+  admitP (~ (contains h1 y));
   assert false //should fail
 
 (* ******************************************************************************** *)
